A better way to setup PCAs.

PartialCombinatoryAlgebras/Basic.lean
@@ -2,109 +2,93 @@ import Mathlib.Data.Part
 
 /-- A partial binary operation on a set. -/
 class PartialApplication (A : Type*) where
-  /-- partial binary application -/
-  app : A → A → Part A
+  /-- partial application -/
+  app : Part A → Part A → Part A
+
+/-- a partial element is defined, with explicit carrier -/
+notation:50 u:max " ⇓ " => Part.Dom u
 
 @[inherit_doc]
-infixr:30 "•" => PartialApplication.app
-
-/-- When a set is equipped with a partial application, we allow implicit
-    coercions from the set to its partial elements. -/
-instance PartialApplication.hasCoe {A} [PartialApplication A]: Coe A (Part A) where
-  coe := Part.some
-
-/-- Monadic application that can be used for expressions with nested applications. -/
-@[reducible]
-def PartialApplication.mul {A} [PartialApplication A] (a b : Part A) : Part A :=
-  Part.bind a (fun u => Part.bind b (fun v => app u v))
-
-instance PartialApplication.hasMul {A} [PartialApplication A]: Mul (Part A) where
-  mul := mul
-
-/-- Applicative expressions over a context of variables `Γ` and constants `A`. -/
-inductive Expr (Γ : Type*) (A : Type*) where
-  /-- An element as an expression -/
-| elm : A → Expr Γ A
-  /-- A variable as an expression -/
-| var : Γ → Expr Γ A
-  /-- Formal application of expressions -/
-| app : Expr Γ A → Expr Γ A → Expr Γ A
-
-instance Expr.hasMul {Γ A} : Mul (Expr Γ A) where mul := Expr.app
-
-/-- Applicative expressions equipped with the partial application operation `Expr.app`,
-    which happens to be total. -/
-instance Expr.partialApplication {Γ A : Type*} : PartialApplication (Expr Γ A) where
-  app e₁ e₂ := e₁.app e₂
-
-section Expressions
-
-variable {A : Type*} [PartialApplication A]
-variable {Γ : Type*}
-
-/-- The evaluation of an expression with respect to a partial application
-    and valuation of the variables. -/
-def Expr.eval : Expr Γ A → (Γ → A) → Part A
-| .elm a, _ => a
-| .var x, η => η x
-| .app e₁ e₂, η => do
-  let v₁ ← eval e₁ η
-  let v₂ ← eval e₂ η
-  v₁ • v₂
-
-@[inherit_doc]
-notation " ⟦" e "⟧ " η => Expr.eval e η
-
-/-- The statement that an expression is defined for the given valuation. -/
-def Expr.defined (e : Expr Γ A) (η : Γ → A) := (⟦ e ⟧ η).Dom
-
-@[inherit_doc]
-notation:40 e:40 "↓" η:40 => Expr.defined e η
-
-/-- The statement that an expression is undefined for the given valuation. -/
-def Expr.undefined (e : Expr Γ A) (η : Γ → A) := ¬ (⟦ e ⟧ η).Dom
-
-@[inherit_doc]
-notation e "↑" η:40 => Expr.undefined e η
-
-/-- The left-hand argument of an application is defined if the application is defined. -/
-theorem Expr.defined_left {e₁ e₂ : Expr Γ A} {η : Γ → A} : (e₁.app e₂) ↓ η → e₁ ↓ η := by
-  rintro ⟨_, _⟩
-  assumption
-
-/-- The right-hand argument of an application is defined if the application is defined. -/
-theorem Expr.defined_right {e₁ e₂ : Expr Γ A} {η : Γ → A} : (.app e₁ e₂) ↓ η → (e₂ ↓ η) := by
-  rintro ⟨_, ⟨_, _⟩⟩
-  assumption
-
-end Expressions
+infixl:70 (priority := high) " ⬝ " => PartialApplication.app
 
 /-- The partial combinatory structure on a set `A`. -/
 class PCA (A : Type*) extends PartialApplication A where
-  K : A
-  S : A
-  defined_K₁ : ∀ a, (K • a).Dom
-  defined_S₁ : ∀ a, (S • a).Dom
-  defined_S₂ : ∀ a b, ((S • a).get (defined_S₁ a) • b).Dom
-  eq_K : ∀ (a b : A), (K : Part A) * a * b = a
-  eq_S : ∀ (a b c : A), (S : Part A) * a * b * c = (a * b) * (a * c)
-
-notation "𝕜" => Part.some PCA.K
-notation "𝕤" => Part.some PCA.S
+  K : Part A
+  S : Part A
+  defined_K₀ : K ⇓
+  defined_K₁ : ∀ {u : Part A}, u ⇓ → (K ⬝ u) ⇓
+  defined_S₀ : S ⇓
+  defined_S₁ : ∀ {u : Part A}, u ⇓ → (S ⬝ u) ⇓
+  defined_S₂ : ∀ {u v : Part A}, u ⇓ → v ⇓ → (S ⬝ u ⬝ v) ⇓
+  eq_K : ∀ (u v : Part A), u ⇓ → v ⇓ → (K ⬝ u ⬝ v) = u
+  eq_S : ∀ (u v w : Part A), u ⇓ → v ⇓ → w ⇓ → S ⬝ u ⬝ v ⬝ w = (u ⬝ w) ⬝ (v ⬝ w)
 
 namespace PCA
 
 variable {A : Type*} [PCA A]
 
-lemma definedS (a b : A) : (𝕤 * (a : Part A) * (b : Part A)).Dom := by
-  simp [HMul.hMul, Mul.mul, Part.bind_dom]
-  use (defined_S₁ a)
-  use (defined_S₂ a b)
+@[reducible]
+def I : Part A := S ⬝ K ⬝ K
 
-lemma definedK1 (a : A) : (𝕜 * (a : Part A)).Dom := by
-  simp [HMul.hMul, Mul.mul, Part.bind_dom]
-  use (defined_K₁ a)
+lemma defined_I : (I : Part A) ⇓ := by
+  apply defined_S₂ <;> apply defined_K₀
 
-def id : A := (𝕤 * 𝕜 * 𝕜 : Part A).get (definedS _ _)
+lemma eq_I {u : Part A} : u ⇓ → I ⬝ u = u := by
+  intro du
+  simp [I, eq_S, eq_K, defined_K₀, defined_K₁, du]
 
 end PCA
+
+inductive Expr (Γ A : Type*) where
+| K : Expr Γ A
+| S : Expr Γ A
+| elm : A → Expr Γ A
+| var : Γ → Expr Γ A
+| app : Expr Γ A → Expr Γ A → Expr Γ A
+
+inductive Extend (Γ : Type*) where
+| here : Extend Γ
+| there : Γ → Extend Γ
+
+def extend {Γ A : Type} (η : Γ → A) (a : A) : Extend Γ → A
+| .here => a
+| .there x => η x
+
+namespace Expr
+
+  /-- The evaluation of an expression with respect to a partial application
+      and valuation of the variables. -/
+  def eval {Γ A} [PCA A]: Expr Γ A → (Γ → A) → Part A
+  | .K, _ => PCA.K
+  | .S, _ => PCA.S
+  | .elm a, _ => .some a
+  | .var x, η => .some (η x)
+  | .app e₁ e₂, η => (eval e₁ η) ⬝ (eval e₂ η)
+
+  @[inherit_doc]
+  notation " ⟦" e "⟧ " η => Expr.eval e η
+
+  def defined {Γ A} [PCA A] (e : Expr Γ A) :=
+    ∀ (η : Γ → A), (⟦ e ⟧ η) ⇓
+
+  def abstr {Γ A} [PCA A] : Expr (Extend Γ) A → Expr Γ A
+  | .K => .app .K .K
+  | .S => .app .K .S
+  | .elm a => .app (.K) (.elm a)
+  | .var (.here) => .app (.app .S .K) .K
+  | .var (.there x) => .app .K (.var x)
+  | .app e₁ e₂ => .app (.app .S (abstr e₁)) (abstr e₂)
+
+  lemma defined_abstr {Γ A} [PCA A] (e : Expr (Extend Γ) A) : defined (abstr e) := by
+    intro η
+    induction e
+    case K => simp [eval, PCA.defined_K₁, PCA.defined_K₀]
+    case S => simp [eval, PCA.defined_S₁, PCA.defined_K₁, PCA.defined_S₀]
+    case elm => simp [eval, PCA.defined_K₁]
+    case var x =>
+      cases x
+      case here => simp [eval, PCA.defined_S₂, PCA.defined_S₁, PCA.defined_K₀]
+      case there => simp [eval, PCA.defined_K₁]
+    case app e₁ e₂ ih₁ ih₂ => simp [eval, PCA.defined_S₂, ih₁, ih₂]
+
+end Expr
